support loop invariants and assert annotations

refinedVST/typing/ClightSugar.v
@@ -7,5 +7,11 @@ Section type.
   Context `{!typeG OK_ty Σ}.
 
   Definition Sannot (a : assert) := Sskip.
+  #[global] Arguments Sannot : simpl never.
+  Global Typeclasses Opaque Sannot.
+
   Definition Sloop (a : assert) s1 s2 := Sloop s1 s2.
+  #[global] Arguments Sloop : simpl never.
+  Global Typeclasses Opaque Sloop.
+
 End type.
