refinedVST/typing/automation.v
@@ -177,6 +177,15 @@ Ltac liRStmt :=
       | Ssequence _ _ => notypeclasses refine (tac_fast_apply (type_seq _ _ _ _ _ _) _)
       | Sreturn $ Some _ => notypeclasses refine (tac_fast_apply (type_return_some _ _ _ _ _) _)
       | Sreturn None => notypeclasses refine (tac_fast_apply (type_return_none _ _ _ _ _) _)
+      | Sskip => notypeclasses refine (tac_fast_apply (type_skips _ _ _ _) _)
+      | Scall _ _ _ => notypeclasses refine (tac_fast_apply (type_call_fnptr _ _ _ _ _ _ _ _ _ _) _); [done|]
+      | Sifthenelse _ _ _ => notypeclasses refine (tac_fast_apply (type_if _ _ _ _ _ _ _) _)
+      | Sloop _ _ _ => notypeclasses refine (tac_fast_apply (type_inv_loop _ _ _ _ _ _ _) _)
+      | Sbreak =>notypeclasses refine (tac_fast_apply (type_break _ _ _ _) _)
+      | Scontinue => notypeclasses refine (tac_fast_apply (type_continue _ _ _ _) _)
+      | Sswitch _ _ => notypeclasses refine (tac_fast_apply (type_switch _ _ _ _ _ _) _)
+      | Slabel _ _ => notypeclasses refine (tac_fast_apply (type_label _ _ _ _ _ _) _)
+      | Sannot _ => notypeclasses refine (tac_fast_apply (type_annot_stmt_assert _ _ _ _ _) _)
       | _ => fail "do_stmt: unknown stmt" s
       end
     end
